coq/handwritten/S2N/Translation/HandshakeAction.v
@@ -1,33 +1,15 @@
-From Bits Require Import operations.
-From Bits Require Import spec.
-
-From Coq Require Import Lists.List.
-From Coq Require Import String.
-From Coq Require Import Program.Equality.
-From Coq Require Import Vector.
-
 From CryptolToCoq Require Import CryptolPrimitivesForSAWCore.
 From CryptolToCoq Require Import CryptolPrimitivesForSAWCoreExtra.
-From CryptolToCoq Require Import SAWCorePrelude.
-From CryptolToCoq Require Import SAWCorePrelude_proofs.
-From CryptolToCoq Require Import SAWCoreScaffolding.
-From CryptolToCoq Require Import SAWCoreVectorsAsCoqVectors.
-From CryptolToCoq Require Import S2N.
-From CryptolToCoq Require Import S2N.Embedding.
-From CryptolToCoq Require Import S2N.Pointed.
 
-From mathcomp Require Import eqtype.
-From mathcomp Require Import fintype.
-From mathcomp Require Import seq.
-From mathcomp Require Import ssreflect.
-From mathcomp Require Import ssrbool.
-From mathcomp Require Import ssrnat.
+From S2N Require Import Embedding.
+From S2N Require Import Pointed.
+
 From mathcomp Require Import tuple.
 
 Import CryptolPrimitives.
-Import ListNotations.
-Import SAWCorePrelude.
-Import VectorNotations.
+
+Definition cry_handshake_action : Type
+  := (seq 8 bool * (seq 8 bool * seq 8 bool)).
 
 Record HandshakeAction := MkHandshakeAction
   {
@@ -37,32 +19,32 @@ Record HandshakeAction := MkHandshakeAction
   }.
 
 Global Instance Embedding_HandshakeAction
-  : Embedding (seq 8 bool * (seq 8 bool * seq 8 bool)) HandshakeAction :=
-  {|
-    toAbstract :=
-      fun '(a, (b, c)) =>
-        {|
-          messageType := toAbstract a; (* Cryptol sorts the fields *)
-          recordType  := toAbstract b;
-          writer      := toAbstract c;
-        |}
-    ;
-    toConcrete :=
-      fun c =>
-        ( toConcrete (messageType c)
-        , ( toConcrete (recordType c)
-          , toConcrete (writer c)
+    : Embedding cry_handshake_action HandshakeAction :=
+    {|
+      toAbstract :=
+        fun '(a, (b, c)) =>
+          {|
+            messageType := toAbstract a; (* Cryptol sorts the fields *)
+            recordType  := toAbstract b;
+            writer      := toAbstract c;
+          |}
+      ;
+      toConcrete :=
+        fun c =>
+          ( toConcrete (messageType c)
+            , ( toConcrete (recordType c)
+                , toConcrete (writer c)
+            )
           )
-        )
-    ;
-  |}.
+      ;
+    |}.
 
-Global Instance Pointed_HandshakeAction : Pointed HandshakeAction :=
-  {|
-    pointed :=
-      {|
-        recordType  := pointed;
-        messageType := pointed;
-        writer      := pointed;
-      |};
-  |}.
+  Global Instance Pointed_HandshakeAction : Pointed HandshakeAction :=
+    {|
+      pointed :=
+        {|
+          recordType  := pointed;
+          messageType := pointed;
+          writer      := pointed;
+        |};
+    |}.
