coq/handwritten/Lift/HandshakeAction.v
@@ -1,0 +1,496 @@
+From CryptolToCoq Require Import CryptolPrimitivesForSAWCore.
+From CryptolToCoq Require Import CryptolPrimitivesForSAWCoreExtra.
+From CryptolToCoq Require Import SAWCorePrelude.
+From CryptolToCoq Require Import SAWCorePrelude_proofs.
+From CryptolToCoq Require Import SAWCoreScaffolding.
+From CryptolToCoq Require Import SAWCoreVectorsAsCoqVectors.
+
+From Coq Require Import Vectors.Vector.
+
+(* From mathcomp Require Import seq. *)
+(* From mathcomp Require Import tuple. *)
+
+From S2N Require Import S2N.
+
+From Ornamental Require Import Ornaments.
+
+Set DEVOID search prove equivalence. (* <-- Correctness proofs for search *)
+Set DEVOID lift type. (* <-- Prettier types than the ones Coq infers *)
+
+(* Import CryptolPrimitives. *)
+(* (* Import ListNotations. *) *)
+(* Import SAWCorePrelude. *)
+(* (* Import VectorNotations. *) *)
+
+(* Definition seq : Num -> (Type) -> Type := *)
+(*   (fun (num : ((@Num))) (a : Type) => *)
+(*    ((@Num_rect) *)
+(*     ((fun (num : ((@Num))) => Type)) *)
+(*     ((fun (n : ((@Nat))) => *)
+(*       ((@SAWCoreVectorsAsCoqVectors.Vec) (n) (a)))) *)
+(*     (((@Stream) (a))) (num))). *)
+
+(* When those two lines are commented out, the lifting of [get_record_type]
+works! *)
+
+Import CryptolPrimitives.
+
+Module HandshakeAction.
+
+  Definition cry_handshake_action : Type
+    := (seq 8 bool * (seq 8 bool * seq 8 bool)).
+
+  Record HandshakeAction :=
+    MkHandshakeAction
+    {
+    recordType  : seq 8 bool;
+    messageType : seq 8 bool;
+    writer      : seq 8 bool;
+    }.
+
+  Scheme Induction for HandshakeAction Sort Prop.
+  Scheme Induction for HandshakeAction Sort Type.
+  Scheme Induction for HandshakeAction Sort Set.
+
+  Definition get_record_type (ha : cry_handshake_action) : seq 8 bool :=
+    fst ha.
+
+  Definition get_message_type (ha : cry_handshake_action) : seq 8 bool :=
+    Prod.fst _ _ (Prod.snd _ _ ha).
+
+  Definition get_writer (ha : cry_handshake_action) : seq 8 bool :=
+    Prod.snd _ _ (Prod.snd _ _ ha).
+
+  Definition MY_CLIENT_HELLO : (seq 8 bool * (seq 8 bool * seq 8 bool)) :=
+    mkAct (TLS_HANDSHAKE (seq 8 Bool) (PLiteralSeqBool 8))
+          (TLS_CLIENT_HELLO (seq 8 Bool) (PLiteralSeqBool 8))
+          (ecNumber 67 (seq 8 Bool) (PLiteralSeqBool 8)).
+
+End HandshakeAction.
+
+Preprocess Module HandshakeAction
+  as HandshakeAction'
+     { opaque
+       seq
+     }.
+
+Lift HandshakeAction'.cry_handshake_action
+     HandshakeAction'.HandshakeAction
+  in HandshakeAction'.get_record_type
+  as getRecordType.
+
+Lift HandshakeAction'.cry_handshake_action
+     HandshakeAction'.HandshakeAction
+  in HandshakeAction'.get_message_type
+  as getMessageType.
+
+Lift HandshakeAction'.cry_handshake_action
+     HandshakeAction'.HandshakeAction
+  in HandshakeAction'.get_writer
+  as getWriter.
+
+Lift HandshakeAction'.cry_handshake_action
+     HandshakeAction'.HandshakeAction
+  in HandshakeAction'.MY_CLIENT_HELLO
+  as clientHello.
+
+Theorem checkMessageType
+  : getMessageType clientHello
+    = HandshakeAction.get_message_type HandshakeAction.MY_CLIENT_HELLO.
+Proof.
+  reflexivity.
+Qed.
+
+Theorem checkRecordType
+  : getRecordType clientHello
+    =
+    HandshakeAction.get_record_type HandshakeAction.MY_CLIENT_HELLO.
+Proof.
+  reflexivity.
+Qed.
+
+Theorem checkWriter
+  : getWriter clientHello
+    =
+    HandshakeAction.get_writer HandshakeAction.MY_CLIENT_HELLO.
+Proof.
+  reflexivity.
+Qed.
+
+From Lift Require Import S2N.
+
+Check S2N'.state_machine_fn.
+
+Lift HandshakeAction'.cry_handshake_action
+     HandshakeAction'.HandshakeAction
+  in S2N'.mkAct
+  as mkAct'.
+
+Lift HandshakeAction'.cry_handshake_action
+     HandshakeAction'.HandshakeAction
+  in S2N'.TLS_HANDSHAKE
+  as TLS_HANDSHAKE'.
+
+Lift HandshakeAction'.cry_handshake_action
+     HandshakeAction'.HandshakeAction
+  in S2N'.TLS_CLIENT_HELLO
+  as TLS_CLIENT_HELLO'.
+
+Lift HandshakeAction'.cry_handshake_action
+     HandshakeAction'.HandshakeAction
+  in PLiteralSeqBool
+  as PLiteralSeqBool'.
+
+Lift HandshakeAction'.cry_handshake_action
+     HandshakeAction'.HandshakeAction
+  in PCmp
+  as PCmpP
+     { opaque
+       Records.CoreRecords.Fields
+       Records.CoreRecords.ascii_to_p
+       Records.CoreRecords.bool_to_p
+       Records.CoreRecords.fields_get
+       Records.CoreRecords.fields_insert
+       Records.CoreRecords.fields_leaf
+       Records.CoreRecords.fields_join
+       Records.CoreRecords.fields_singleton
+       Records.CoreRecords.get_member
+       Records.CoreRecords.record_empty
+       Records.CoreRecords.record_get
+       Records.CoreRecords.record_here
+       Records.CoreRecords.record_left
+       Records.CoreRecords.record_right
+       Records.CoreRecords.record_singleton
+       Records.CoreRecords.Rjoin
+       Records.CoreRecords.string_to_p
+     }.
+
+Lift HandshakeAction'.cry_handshake_action
+     HandshakeAction'.HandshakeAction
+  in PCmpWord
+  as PCmpWordP
+     { opaque
+       Records.CoreRecords.Fields
+       Records.CoreRecords.ascii_to_p
+       Records.CoreRecords.bool_to_p
+       Records.CoreRecords.fields_get
+       Records.CoreRecords.fields_insert
+       Records.CoreRecords.fields_leaf
+       Records.CoreRecords.fields_join
+       Records.CoreRecords.fields_singleton
+       Records.CoreRecords.get_member
+       Records.CoreRecords.record_empty
+       Records.CoreRecords.record_get
+       Records.CoreRecords.record_here
+       Records.CoreRecords.record_left
+       Records.CoreRecords.record_right
+       Records.CoreRecords.record_singleton
+       Records.CoreRecords.Rjoin
+       Records.CoreRecords.string_to_p
+       bvCmp
+     }.
+
+Lift HandshakeAction'.cry_handshake_action
+     HandshakeAction'.HandshakeAction
+  in PCmpSeqBool
+  as PCmpSeqBool'.
+
+Lift HandshakeAction'.cry_handshake_action
+     HandshakeAction'.HandshakeAction
+  in ecNumber
+  as ecNumber'.
+
+Lift HandshakeAction'.cry_handshake_action
+     HandshakeAction'.HandshakeAction
+  in ecZero
+  as ..P.
+
+Lift HandshakeAction'.cry_handshake_action
+     HandshakeAction'.HandshakeAction
+  in ecEq
+  as ecEq'
+     { opaque
+       Records.CoreRecords.Fields
+       Records.CoreRecords.ascii_to_p
+       Records.CoreRecords.bool_to_p
+       Records.CoreRecords.fields_get
+       Records.CoreRecords.fields_insert
+       Records.CoreRecords.fields_leaf
+       Records.CoreRecords.fields_join
+       Records.CoreRecords.fields_singleton
+       Records.CoreRecords.get_member
+       Records.CoreRecords.record_empty
+       Records.CoreRecords.record_get
+       Records.CoreRecords.record_here
+       Records.CoreRecords.record_left
+       Records.CoreRecords.record_right
+       Records.CoreRecords.record_singleton
+       Records.CoreRecords.Rjoin
+       Records.CoreRecords.string_to_p
+     }.
+
+Lift HandshakeAction'.cry_handshake_action
+     HandshakeAction'.HandshakeAction
+  in S2N'.TLS_SERVER_SESSION_LOOKUP
+  as TLS_SERVER_SESSION_LOOKUP'.
+
+Lift HandshakeAction'.cry_handshake_action
+     HandshakeAction'.HandshakeAction
+  in S2N'.TLS_SERVER_HELLO
+  as TLS_SERVER_HELLO'.
+
+Lift HandshakeAction'.cry_handshake_action
+     HandshakeAction'.HandshakeAction
+  in S2N'.TLS_SERVER_NEW_SESSION_TICKET
+  as TLS_SERVER_NEW_SESSION_TICKET'.
+
+Lift HandshakeAction'.cry_handshake_action
+     HandshakeAction'.HandshakeAction
+  in S2N'.TLS_SERVER_CERT
+  as TLS_SERVER_CERT'.
+
+Lift HandshakeAction'.cry_handshake_action
+     HandshakeAction'.HandshakeAction
+  in S2N'.TLS_SERVER_CERT_STATUS
+  as TLS_SERVER_CERT_STATUS'.
+
+Lift HandshakeAction'.cry_handshake_action
+     HandshakeAction'.HandshakeAction
+  in S2N'.TLS_SERVER_KEY
+  as TLS_SERVER_KEY'.
+
+Lift HandshakeAction'.cry_handshake_action
+     HandshakeAction'.HandshakeAction
+  in S2N'.TLS_SERVER_CERT_REQ
+  as TLS_SERVER_CERT_REQ'.
+
+Lift HandshakeAction'.cry_handshake_action
+     HandshakeAction'.HandshakeAction
+  in S2N'.TLS_SERVER_HELLO_DONE
+  as TLS_SERVER_HELLO_DONE'.
+
+Lift HandshakeAction'.cry_handshake_action
+     HandshakeAction'.HandshakeAction
+  in S2N'.TLS_CLIENT_CERT
+  as TLS_CLIENT_CERT'.
+
+Lift HandshakeAction'.cry_handshake_action
+     HandshakeAction'.HandshakeAction
+  in S2N'.TLS_CLIENT_KEY
+  as TLS_CLIENT_KEY'.
+
+Lift HandshakeAction'.cry_handshake_action
+     HandshakeAction'.HandshakeAction
+  in S2N'.TLS_CLIENT_CERT_VERIFY
+  as TLS_CLIENT_CERT_VERIFY'.
+
+Lift HandshakeAction'.cry_handshake_action
+     HandshakeAction'.HandshakeAction
+  in S2N'.TLS_CHANGE_CIPHER_SPEC
+  as TLS_CHANGE_CIPHER_SPEC'.
+
+Lift HandshakeAction'.cry_handshake_action
+     HandshakeAction'.HandshakeAction
+  in S2N'.TLS_CLIENT_FINISHED
+  as TLS_CLIENT_FINISHED'.
+
+Lift HandshakeAction'.cry_handshake_action
+     HandshakeAction'.HandshakeAction
+  in S2N'.TLS_SERVER_FINISHED
+  as TLS_SERVER_FINISHED'.
+
+Lift HandshakeAction'.cry_handshake_action
+     HandshakeAction'.HandshakeAction
+  in S2N'.TLS_APPLICATION_DATA
+  as TLS_APPLICATION_DATA'.
+
+Lift HandshakeAction'.cry_handshake_action
+     HandshakeAction'.HandshakeAction
+  in S2N'.state_machine_fn
+  as stateMachineFn.
+
+Compute getRecordType
+        (stateMachineFn
+         (S2N'.CLIENT_HELLO
+          (seq 5 bool)
+          ((@CryptolPrimitives.PLiteralSeqBool) (((@TCNum) (5))))
+         )
+        ) = HandshakeAction'.get_record_type
+            (S2N'.state_machine_fn
+             (S2N'.CLIENT_HELLO
+              (seq 5 bool)
+              ((@CryptolPrimitives.PLiteralSeqBool) (((@TCNum) (5))))
+             )
+            ).
+
+Lift HandshakeAction'.cry_handshake_action
+     HandshakeAction'.HandshakeAction
+  in S2N'.state_machine
+  as stateMachine.
+
+
+Lift HandshakeAction'.cry_handshake_action
+     HandshakeAction'.HandshakeAction
+  in S2N'.
+  as '.
+
+Lift HandshakeAction'.cry_handshake_action
+     HandshakeAction'.HandshakeAction
+  in S2N'.
+  as '.
+
+Lift HandshakeAction'.cry_handshake_action
+     HandshakeAction'.HandshakeAction
+  in S2N'.
+  as '.
+
+Lift HandshakeAction'.cry_handshake_action
+     HandshakeAction'.HandshakeAction
+  in S2N'.
+  as '.
+
+Check (S2N'.TLS_HANDSHAKE).
+
+Lift HandshakeAction'.cry_handshake_action
+     HandshakeAction'.HandshakeAction
+  in S2N'.state_machine
+  as stateMachine
+     { opaque
+       Bits.spec.spec.low
+       Coq.Arith.PeanoNat.Nat.even
+       Records.CoreRecords.Fields
+       Records.CoreRecords.ascii_to_p
+       Records.CoreRecords.bool_to_p
+       Records.CoreRecords.fields_get
+       Records.CoreRecords.fields_insert
+       Records.CoreRecords.fields_leaf
+       Records.CoreRecords.fields_join
+       Records.CoreRecords.fields_singleton
+       Records.CoreRecords.get_member
+       Records.CoreRecords.record_empty
+       Records.CoreRecords.record_get
+       Records.CoreRecords.record_here
+       Records.CoreRecords.record_left
+       Records.CoreRecords.record_right
+       Records.CoreRecords.record_singleton
+       Records.CoreRecords.Rjoin
+       Records.CoreRecords.string_to_p
+       Records.Notation.Rget
+       CryptolToCoq.SAWCoreScaffolding.error
+       SAWCorePrelude.bvToInt
+       SAWCorePrelude.intToBv
+       mathcomp.ssreflect.eqtype.eq_irrelevance
+       mathcomp.ssreflect.ssrnat.half
+       mathcomp.ssreflect.tuple.behead_tupleP
+       CryptolPrimitives.seq
+       CryptolPrimitives.seqMap
+       CryptolPrimitives.ecFromTo
+       CryptolPrimitives.PLiteralSeqBool
+       CryptolPrimitives.tcAdd
+       CryptolPrimitives.tcSub
+       CryptolPrimitives.seq_cong1
+       SAWCoreScaffolding.Bool
+       SAWCoreScaffolding.coerce
+     } .
+
+Local Open Scope form_scope.
+
+
+
+
+
+Definition ACTIVE_MESSAGE (conn : ((prod) (@SAWCoreScaffolding.Bool) (((prod)
+(((@CryptolPrimitives.seq) (((@TCNum) (2))) (@SAWCoreScaffolding.Bool)))
+(((prod) (((@CryptolPrimitives.seq) (((@TCNum) (8)))
+(@SAWCoreScaffolding.Bool))) (((prod) (((prod) (((@CryptolPrimitives.seq)
+(((@TCNum) (32))) (@SAWCoreScaffolding.Bool))) (((@CryptolPrimitives.seq)
+(((@TCNum) (32))) (@SAWCoreScaffolding.Bool))))) (((prod)
+(@SAWCoreScaffolding.Bool) (((prod) (@SAWCoreScaffolding.Bool) (((prod)
+(((@CryptolPrimitives.seq) (((@TCNum) (32))) (@SAWCoreScaffolding.Bool)))
+(((prod) (@SAWCoreScaffolding.Bool) (@SAWCoreScaffolding.Bool)))))))))))))))))
+:= ((@CryptolPrimitives.ecAt) (((@TCNum) (32))) (((@CryptolPrimitives.seq)
+(((@TCNum) (32))) (@SAWCoreScaffolding.Bool))) (((@TCNum) (32)))
+(((@CryptolPrimitives.ecAt) (((@TCNum) (128))) (((@CryptolPrimitives.seq)
+(((@TCNum) (32))) (((@CryptolPrimitives.seq) (((@TCNum) (32)))
+(@SAWCoreScaffolding.Bool))))) (((@TCNum) (32))) (handshakes) (((fst) (((fst)
+(((snd) (((snd) (((snd) (conn))))))))))))) (((snd) (((fst) (((snd) (((snd)
+(((snd) (conn)))))))))))).
+
+Definition ACTIVE_STATE (conn : ((prod) (@SAWCoreScaffolding.Bool) (((prod)
+(((@CryptolPrimitives.seq) (((@TCNum) (2))) (@SAWCoreScaffolding.Bool)))
+(((prod) (((@CryptolPrimitives.seq) (((@TCNum) (8)))
+(@SAWCoreScaffolding.Bool))) (((prod) (((prod) (((@CryptolPrimitives.seq)
+(((@TCNum) (32))) (@SAWCoreScaffolding.Bool))) (((@CryptolPrimitives.seq)
+(((@TCNum) (32))) (@SAWCoreScaffolding.Bool))))) (((prod)
+(@SAWCoreScaffolding.Bool) (((prod) (@SAWCoreScaffolding.Bool) (((prod)
+(((@CryptolPrimitives.seq) (((@TCNum) (32))) (@SAWCoreScaffolding.Bool)))
+(((prod) (@SAWCoreScaffolding.Bool) (@SAWCoreScaffolding.Bool)))))))))))))))))
+:= ((@CryptolPrimitives.ecAt) (((@TCNum) (17))) (((prod)
+(((@CryptolPrimitives.seq) (((@TCNum) (8))) (@SAWCoreScaffolding.Bool)))
+(((prod) (((@CryptolPrimitives.seq) (((@TCNum) (8)))
+(@SAWCoreScaffolding.Bool))) (((@CryptolPrimitives.seq) (((@TCNum) (8)))
+(@SAWCoreScaffolding.Bool))))))) (((@TCNum) (32))) (state_machine)
+(((ACTIVE_MESSAGE) (conn)))).
+
+Fixpoint seq_to_tuple {T} {n : nat} (s : seq n T) : n.-tuple T :=
+  match s with
+  | nil => [tuple]
+  | cons h _ t => cat_tuple [tuple of [:: h]] (seq_to_tuple t)
+  end.
+
+Fixpoint tuple_to_seq {T} {n : nat} (t : n.-tuple T) : seq n T.
+  move : n t.
+  match t with
+  |  => Vector.nil
+  end.
+
+
+
+
+
+
+
+
+
+
+Lift HandshakeAction'.cry_handshake_action
+     HandshakeAction'.HandshakeAction'
+  in S2N'.ACTIVE_STATE
+  as stateMachineFn
+     { opaque
+       S2N'.CryptolToCoq_CryptolPrimitivesForSAWCore_CryptolPrimitives_ecAt
+       S2N'.ACTIVE_MESSAGE
+       CryptolPrimitives.seq
+     }.
+
+Print 42.
+
+(*
+
+// A model of the handshake states (array state_machine in C)
+state_machine : [17]handshake_action
+state_machine = [state_machine_fn m | m <- [0..16]]
+
+// Function that tells a handshake_action for a given state
+state_machine_fn : [5] -> handshake_action
+state_machine_fn m =
+  if      m == CLIENT_HELLO then mkAct TLS_HANDSHAKE TLS_CLIENT_HELLO 'C'
+  else if m == SERVER_SESSION_LOOKUP then mkAct TLS_HANDSHAKE TLS_SERVER_SESSION_LOOKUP 'A'
+  else if m == SERVER_HELLO then mkAct TLS_HANDSHAKE TLS_SERVER_HELLO 'S'
+  else if m == SERVER_NEW_SESSION_TICKET then mkAct TLS_HANDSHAKE TLS_SERVER_NEW_SESSION_TICKET 'S'
+  else if m == SERVER_CERT then mkAct TLS_HANDSHAKE TLS_SERVER_CERT 'S'
+  else if m == SERVER_CERT_STATUS then mkAct TLS_HANDSHAKE TLS_SERVER_CERT_STATUS 'S'
+  else if m == SERVER_KEY then mkAct TLS_HANDSHAKE TLS_SERVER_KEY 'S'
+  else if m == SERVER_CERT_REQ then mkAct TLS_HANDSHAKE TLS_SERVER_CERT_REQ 'S'
+  else if m == SERVER_HELLO_DONE then mkAct TLS_HANDSHAKE TLS_SERVER_HELLO_DONE 'S'
+  else if m == CLIENT_CERT then mkAct TLS_HANDSHAKE TLS_CLIENT_CERT 'C'
+  else if m == CLIENT_KEY then mkAct TLS_HANDSHAKE TLS_CLIENT_KEY 'C'
+  else if m == CLIENT_CERT_VERIFY then mkAct TLS_HANDSHAKE TLS_CLIENT_CERT_VERIFY 'C'
+  else if m == CLIENT_CHANGE_CIPHER_SPEC then mkAct TLS_CHANGE_CIPHER_SPEC 0 'C'
+  else if m == CLIENT_FINISHED then mkAct TLS_HANDSHAKE TLS_CLIENT_FINISHED 'C'
+  else if m == SERVER_CHANGE_CIPHER_SPEC then mkAct TLS_CHANGE_CIPHER_SPEC 0 'S'
+  else if m == SERVER_FINISHED then mkAct TLS_HANDSHAKE TLS_SERVER_FINISHED 'S'
+  else if m == APPLICATION_DATA then mkAct TLS_APPLICATION_DATA 0 'B'
+  else zero
+
+ *)
